theories/base.v
@@ -1,2 +1,13 @@
 From Coq Require Export ssreflect.
 Require Export stdpp.prelude.
+
+Definition LEM (P : Prop) := P ∨ ¬ P.
+
+Lemma snoc_inv {A} (l : list A):
+  l = [] ∨ ∃ x l', l = l' ++ [x].
+Proof.
+  destruct l as [|x l']. by left. right.
+  elim: l' x => //. move => x. by eexists _, [].
+  move => x ? IH x'. move: (IH x) => [x'' [l'' ->]].
+  eexists x'', _. by apply: app_comm_cons.
+Qed.
